\chapter{Binomial coefficients are (almost) never powers}


\begin{theorem}[Sylvester's theorem]
    \label{sylvester}
    \lean{chapter3.sylvester}
    \leanok
    For all positive natural \(n, k\) such that \(n \ge 2k\), at least one of the numbers
    \(n, n - 1, \dots, n - k + 1\) has a prime divisor $p$ greater than $k$,
    or, equivalently the binomial coefficient
    \(\binom{n}{k}\) always has a prime factor \(p > k\).
\end{theorem}
\begin{proof}
    TODO
\end{proof}


\begin{theorem}[Binomial coefficients are (almost) never powers]
    \label{binomial_never_powers}
    \lean{chapter3.binomials_coefficients_never_powers}
    \leanok
    The equation \(\binom n k = m ^ l\) has no integer solutions with
    \(l \ge 2\) and \(4 \le k \le n - 4\).
\end{theorem}
\begin{proof}
    \uses{sylvester}
    Note first that we may assume \(n \ge 2k\) because of \(\binom{n}{k} = \binom{n}{n-k}\).
    Suppose the theorem is false, and that \(\binom{n}{k} = m^\ell\).
    The proof, by contradiction, proceeds in the following four steps.
    \begin{enumerate}
    \item By Sylvester's theorem \ref{sylvester}, there is a prime factor \(p\) of \(\binom{n}{k}\) greater than \(k\),
          hence \(p^\ell\) divides \(n(n - 1) \dots (n - k + 1)\). Clearly, only one of the factors \(n - i\)
          can be a multiple of \(p\) (because \(p > k\)), and we conclude \(p^\ell \mid n - i\), and therefore
          \[
          n \ge p^\ell > k^\ell \ge k^2.
          \]
    \item Consider any factor \(n - j\) of the numerator and write it in the form \(n - j = a_j m_j^\ell\),
          where \(a_j\) is not divisible by any nontrivial \(\ell\)-th power.
          We note by (1) that \(a_j\) has only prime divisors less than or equal to \(k\).
          We want to show next that \(a_i \ne a_j\) for \(i \ne j\).
          Assume to the contrary that \(a_i = a_j\) for some \(i < j\). Then \(m_i \ge m_j + 1\) and
        \begin{align*}
        k &> (n - i) - (n - j) = a_j(m_i^\ell - m_j^\ell) \ge a_j((m_j + 1)^\ell - m_j^\ell)\\
          &> a_j \ell m_j^{\ell-1} \ge \ell (a_j m_j^\ell)^{1/2} \ge \ell (n - k + 1)^{1/2}\\
          &\ge \ell \left(\frac{n}{2} + 1\right)^{1/2} > n^{1/2},
        \end{align*}
        which contradicts \(n > k^2\) from above.
    \item Next we prove that the \(a_i\)'s are the integers \(1, 2, \dots, k\) in some order.
    (According to Erd≈ës, this is the crux of the proof.)
    Since we already know that they are all distinct, it suffices to prove that
   \[
   a_0 a_1 \cdots a_{k-1} \text{ divides } k!.
   \]
   Substituting \(n - j = a_j m_j^\ell\) into the equation \(\binom{n}{k} = m^\ell\), we obtain
   \[
   a_0 a_1 \cdots a_{k-1} (m_0 m_1 \cdots m_{k-1})^\ell = k! m^\ell.
   \]
   Canceling the common factors of \(m_0 \cdots m_{k-1}\) and \(m\) yields
   \[
   a_0 a_1 \dots a_{k-1} u^\ell = k! v^\ell
   \]
   with \(\gcd(u, v) = 1\). It remains to show that \(v = 1\). If not, then \(v\) contains a prime divisor \(p\).
   Since \(\gcd(u, v) = 1\), \(p\) must be a prime divisor of \(a_0 a_1 \dots a_{k-1}\) and hence is less than or equal to \(k\).
   By the theorem of Legendre, we know that \(k!\) contains \(p\) to the power \(\sum_{i \ge 1} \left\lfloor \frac{k}{p^i} \right\rfloor\).
   We now estimate the exponent of \(p\) in \(n(n - 1) \dots (n - k + 1)\).
    Let \(i\) be a positive integer, and let \(b_1 < b_2 < \dots < b_s\)
    be the multiples of \(p^i\) among \(n, n - 1, \dots, n - k + 1\). Then \(b_s = b_1 + (s - 1)p^i\) and hence
   \[
   (s - 1)p^i = b_s - b_1 \le n - (n - k + 1) = k - 1,
   \]
   which implies
   \[
   s \le \left\lfloor \frac{k - 1}{p^i} \right\rfloor + 1 \le \left\lfloor \frac{k}{p^i} \right\rfloor + 1.
   \]
    So for each \(i\), the number of multiples of \(p^i\) among \(n, \dots, n-k+1\), and hence among the \(a_j\)'s,
    is bounded by \(\left\lfloor \frac{k}{p^i} \right\rfloor + 1\). This implies that the exponent of \(p\) in \(a_0 a_1 \dots a_{k-1}\) is at most

    \[
    \sum_{i=1}^{\ell-1} \left( \left\lfloor \frac{k}{p^i} \right\rfloor + 1 \right)
    \]

    with the reasoning that we used for Legendre's theorem in Chapter 2.
    The only difference is that this time the sum stops at \(i = \ell - 1\), since the \(a_j\)'s contain no \(\ell\)-th powers.

    Taking both counts together, we find that the exponent of \(p\) in \(v^\ell\) is at most

    \[
    \sum_{i=1}^{\ell-1} \left( \left\lfloor \frac{k}{p^i} \right\rfloor + 1 \right) - \sum_{i \ge 1} \left\lfloor \frac{k}{p^i} \right\rfloor \le \ell - 1,
    \]

    and we have our desired contradiction, since \(v^\ell\) is an \(\ell\)-th power.

    This suffices already to settle the case \(\ell = 2\).
    Indeed, since \(k \ge 4\), one of the \(a_i\)'s must be equal to 4,
    but the \(a_i\)'s contain no squares. So let us now assume that \(\ell \ge 3\).

    \item Since \(k \ge 4\), we must have \(a_{i_1} = 1\), \(a_{i_2} = 2\), \(a_{i_3} = 4\) for some \(i_1, i_2, i_3\), that is,
    \[
    n - i_1 = m_1^\ell, \quad n - i_2 = 2m_2^\ell, \quad n - i_3 = 4m_3^\ell.
    \]

    We claim that \((n - i_2)^2 \ne (n - i_1)(n - i_3)\). If not, put \(b = n - i_2\)
    and \(n - i_1 = b - x, n - i_3 = b + y\), where \(0 < |x|, |y| < k\). Hence
    \[
    b^2 = (b - x)(b + y) \quad \text{or} \quad (y - x)b = xy,
    \]
    where \(x = y\) is plainly impossible. Now we have by part (1)
    \[
    |xy| = b |y - x| \ge b > n - k > (k - 1)^2 \ge |xy|,
    \]
    which is absurd.

    So we have \(m_2^2 \ne m_1 m_3\), where we assume \(m_2^2 > m_1 m_3\) (the other case being analogous),
    and proceed to our last chain of inequalities. We obtain

    \begin{align*}
    2(k - 1)n & > n^2 - (n - k + 1)^2 > (n - i_2)^2 - (n - i_1)(n - i_3)\\
     & = 4[m_2^{2\ell} - (m_1 m_3)^\ell] \ge 4[(m_1 m_3 + 1)^\ell - (m_1 m_3)^\ell] \\
     & \ge 4 \ell m_1^{\ell-1} m_3^{\ell-1}.
    \end{align*}

    Since \(\ell \ge 3\) and \(n > k^\ell \ge k^3 > 6k\), this yields
    \begin{align*}
    2(k - 1)n m_1 m_3 & > 4 \ell m_1^\ell m_3^\ell = \ell (n - i_1)(n - i_3) \\
                      & > \ell (n - k + 1)^2 > 3 \left(n - \frac{n}{6}\right)^2 > 2n^2.
    \end{align*}
    Now since \(m_i \le n^{1/\ell} \le n ^{1/3}\) we finally obtain
    \[
    kn^{2/3} \ge km_1m_3 > (k - 1)m_1m_3 > n,
    \]
    or \(k^3 > n\). With this contradiction, the proof is complete. \qedhere
    \end{enumerate}
\end{proof}
